src/PrintType.cpp
@@ -256,6 +256,8 @@ public:
     void VisitFunctionProtoType(const FunctionProtoType* type,
                                 CoqPrinter& print, ClangPrinter& cprint) {
         print.ctor("Tfunction");
+        cprint.printCallingConv(type->getCallConv(), print);
+        print.output() << fmt::nbsp;
         printQualType(type->getReturnType(), print, cprint);
         print.output() << fmt::nbsp;
         print.begin_list();
