theories/lang/cpp/logic/pred.v
@@ -244,7 +244,8 @@ Section with_cpp.
   (** function specifications written in weakest pre-condition style.
    *)
   Record function_spec : Type :=
-    { fs_return : type
+    { fs_cc : calling_conv
+    ; fs_return : type
     ; fs_arguments : list type
     ; fs_spec : thread_info -> list val -> (val -> mpred) -> mpred
     }.
@@ -252,6 +253,6 @@ Section with_cpp.
   Arguments Build_function_spec : clear implicits.
 
   Definition type_of_spec `(fs : function_spec) : type :=
-    normalize_type (Tfunction fs.(fs_return) fs.(fs_arguments)).
+    normalize_type (Tfunction fs.(fs_cc) fs.(fs_return) fs.(fs_arguments)).
 
 End with_cpp.
